Add a stricter subtyping in source; Experiments on Translation.v

coq/coq/Translation.v
@@ -1,13 +1,17 @@
 Require Import LibTactics.
 Require Import Metalib.Metatheory.
-Require Import List. Import ListNotations.
 Require Import Arith Lia.
 Require Import Strings.String.
 Require Import Sorting.Permutation.
 Require Import Sorting.Sorted.
+Require Import Sorting.Mergesort.
+Require Import List Setoid Permutation Sorted Orders OrdersEx.
+Require Import StructTact.StringOrders.
+Import IfNotations.
+Require Export syntax_ott.
 Require Export Infrastructure.
 
-Lemma TEI_dup : forall (ll:tindex) (At Bt Ct Ct' At':ttyp),
+Lemma TEI_dup : forall (ll:string) (At Bt Ct Ct' At':ttyp),
      rec_typ Ct ->
       (   (  Tlookup  ll   Ct  = Some  At'   /\  eqIndTypTarget At' At )    \/   Tlookup  ll   Ct  = None  )  ->
      eqIndTypTarget At Bt ->
@@ -294,7 +298,7 @@ Proof with eauto using TEI_symm, TEI_refl, TEI_trans.
     all: try lookup_concat ll H9; try lookup_concat ll H3...
   - forwards* (?&?&?): IHHE. inverts H3. inverts H11.
     exists. split.
-    all: unify_lookup; lookup_concat ll1 H12; lookup_concat ll2 H12;
+    all: unify_lookup; lookup_concat l1 H12; lookup_concat l2 H12;
       econstructor...
     all: eauto using eqindtyptarget_wf_typ_1, eqindtyptarget_wf_typ_2,
         wf_rcd_concat, rcd_typ_concat_1, rcd_typ_concat_2, rcd_typ_concat_3.
@@ -392,20 +396,6 @@ Qed.
 (*   - applys IHHE. *)
 (* Admitted. *)
 
-
-(* Source types to type indexes *)
-Notation "|| A ||" := (type2index A) (at level 50, A at next level). (* 1 is too high *)
-
-
-(* Concatenate two record types without any checking *)
-
-Fixpoint ttyp_concat_simpl (A: ttyp) (B: ttyp) :=
-  match A with
-  | ttyp_top => B
-  | ttyp_rcd l At Bt => ttyp_rcd l At (ttyp_concat_simpl Bt B)
-  | _ => ttyp_top
-  end.
-
 Lemma lookup_concat_simpl : forall i A B T,
     Tlookup i A = Some T ->
     Tlookup i (ttyp_concat_simpl A B) = Tlookup i A.
@@ -463,43 +453,6 @@ Proof with simpl in *; eauto.
   rewrite IHHRA...
 Qed.
 
-
-
-(* Source types to target types *)
-
-
-Reserved Notation "|[ A ]|" (at level 5, A at next level).
-
-Fixpoint styp2ttyp (A: typ) : ttyp :=
-  match A with
-  | typ_top => ttyp_top
-  | typ_bot => ttyp_rcd (|| A ||) ttyp_bot ttyp_top
-  | typ_base => ttyp_rcd (|| A ||) ttyp_base ttyp_top
-  | typ_arrow B1 B2 => ttyp_rcd (|| A ||) ( ttyp_arrow (|[ B1 ]|) (|[ B2 ]|)) ttyp_top
-  | typ_rcd l A' => ttyp_rcd (|| A ||) (|[ A' ]|) ttyp_top
-  | typ_and A1 A2 => ttyp_concat_simpl (|[ A1 ]|) (|[ A2 ]|)
-  end
-where "|[ A ]|" := (styp2ttyp A).
-
-(* Fixpoint styp2ttyp (A: typ) : ttyp := *)
-(*   match A with *)
-(*   | typ_top => ttyp_top *)
-(*   | typ_bot => ttyp_rcd (|| A ||) ttyp_bot ttyp_top *)
-(*   | typ_base => ttyp_rcd (|| A ||) ttyp_base ttyp_top *)
-(*   | typ_arrow B1 B2 => ttyp_rcd (|| A ||) (ttyp_arrow (|[ B1 ]|) (|[ B2 ]|)) ttyp_top *)
-(*   | typ_rcd l A' => ttyp_rcd (|| A ||) (|[ A' ]|) ttyp_top *)
-(*   | typ_and A1 A2 => ttyp_concat_simpl (|[ A1 ]|) (|[ A2 ]|) *)
-(*   end *)
-(* where "|[ A ]|" := (styp2ttyp A). *)
-
-
-(* Properties of translation (to type index) functions *)
-(* Lemma tindex_trans_arrow : forall A B, *)
-(*     || (typ_arrow A B) || = ti_arrow || B ||. *)
-(* Admitted. *)
-(* Lemma tindex_trans_rcd : forall l A, *)
-(*     || (typ_rcd l A) || = ti_rcd l || A ||. *)
-(* Admitted. *)
 
 (* Properties of translation (to target type) functions *)
 
@@ -595,8 +548,6 @@ Proof with eauto.
 Admitted.
 
 
-
-
 Lemma ttyp_trans_rcd : forall l A,
 (* ord A -> ~ toplike A -> *) (* S-arrow requires no precondition *)
 |[(typ_rcd l A)]| = ttyp_rcd (||(typ_rcd l A)||) |[A]| ttyp_top.
@@ -615,7 +566,7 @@ Admitted.
 
 Fixpoint context_trans (G:ctx) : tctx :=
   match G with
-  | [] => []
+  | nil => nil
   | (x, A) :: l => (x, |[A]|) :: (context_trans l)
   end.
 
@@ -717,3 +668,899 @@ Admitted.
 
 Lemma subtypespec_andr : forall A B, subtype_wrt_lookup |[typ_and A B]| |[B]|.
 Admitted.
+
+(* originally in source5 *)
+
+(* Properties on merge *)
+Locate merge.
+Module Import NSort := Sort NTTLB.
+Lemma merge_empty : forall l,
+    merge nil l = l.
+Proof.
+  introv. induction* l.
+Qed.
+
+Lemma merge_empty_r : forall l,
+    merge l nil = l.
+Proof.
+  introv. induction* l.
+Qed.
+
+#[local] Hint Rewrite merge_empty merge_empty_r : merge.
+
+Lemma merge_cons : forall a l b r,
+    merge (a::l) (b::r) =
+      if if proj1_sig (string_compare_lex a b) is Gt then false else true then a :: merge l (b::r) else b :: merge (a::l) r.
+Proof with eauto.
+  introv. induction* l; destruct (proj1_sig (string_compare_lex a b)); autorewrite with merge...
+Qed.
+
+#[local] Hint Rewrite merge_cons : merge.
+
+
+(** * Multisets *)
+From Coq Require Import FunctionalExtensionality.
+Definition multiset := string -> nat.
+
+(** The [empty] multiset has multiplicity [0] for every value. *)
+
+Definition empty : multiset :=
+  fun x => 0.
+
+(** Multiset [singleton v] contains only [v], and exactly once. *)
+
+Definition singleton (v: string) : multiset :=
+  fun x => if x =? v then 1 else 0.
+
+(** The union of two multisets is their _pointwise_ sum. *)
+
+Definition union (a b : multiset) : multiset :=
+  fun x => a x + b x.
+
+Lemma union_assoc: forall a b c : multiset,
+   union a (union b c) = union (union a b) c.
+Proof.
+  intros.
+  extensionality x.
+  unfolds. eauto using Nat.add_assoc.
+Qed.
+
+Lemma union_comm: forall a b : multiset,
+   union a b = union b a.
+Proof.
+  intros.
+  extensionality x.
+  unfolds. eauto using Nat.add_comm.
+Qed.
+
+Lemma union_swap : forall a b c : multiset,
+    union a (union b c) = union b (union a c).
+Proof.
+  intros.
+  extensionality x.
+  unfolds. lia.
+Qed.
+
+
+Fixpoint contents (al: list string) : multiset :=
+  match al with
+  | nil => empty
+  | a :: bl => union (singleton a) (contents bl)
+  end.
+
+Lemma contents_inv : forall a bl,
+    contents (a :: bl) = union (singleton a) (contents bl).
+Proof.
+  introv. eauto.
+Qed.
+
+Ltac indListSize s :=
+  assert (SizeInd: exists i, s < i) by eauto;
+  destruct SizeInd as [i SizeInd];
+  repeat match goal with | [ h : list _ |- _ ] => (gen h) end;
+  induction i as [|i IH]; [
+    intros; match goal with | [ H : _ < 0 |- _ ] => inverts H end
+  | intros ].
+
+(* prove merge is a permutation *)
+Theorem merge_contents: forall a b,
+    union (contents a) (contents b) = contents (merge a b).
+Proof.
+  intros. extensionality x. indListSize (length a + length b).
+  destruct a; destruct b; autorewrite with merge.
+  (* induction a; induction b; autorewrite with merge. *)
+  1-3: unfolds; simple*.
+  case_if.
+  - simpl. unfold union. rewrite <- IH.
+    unfold union. rewrite (contents_inv s0 b). unfold union.
+    all: simpl in *; lia.
+  - repeat rewrite (contents_inv s0 _). unfold union. rewrite <- IH.
+    { unfold union. lia. }
+    simpl in *; lia.
+Qed.
+
+
+Require Import Ascii.
+Lemma ascii_compare_refl : forall t : ascii, (t ?= t)%char = Eq.
+Proof.
+  intro t. destruct t.
+  unfold Ascii.compare; simpl. rewrite* BinNat.N.compare_refl.
+Qed.
+
+Lemma string_compare_refl : forall s1 : string, (s1 ?= s1) = Eq.
+Proof.
+  intros. induction* s1.
+  simpl. rewrite IHs1. rewrite* ascii_compare_refl.
+Qed.
+
+Check NTTLB.leb_trans.
+(* Lemma new_leb_string_transitive : forall s1 s2 s3 : string, *)
+(*   (s1 <=? s2) = true -> (s2 <=? s3) = true -> (s1 <=? s3) = true. *)
+(* Proof. *)
+(*   intros s1 s2 s3 H1 H2. *)
+(*   pose proof NTTLB.leb_trans. unfolds in H. applys H. *)
+(*   unfolds. unfolds in H1. unfolds in H2. *)
+(*   destruct (s1 ?= s2) eqn:E1; try discriminate; *)
+(*     destruct (s2 ?= s3) eqn:E2; try discriminate. *)
+(*   all: try apply String_as_OT.cmp_eq in E1. *)
+(*   all: try apply String_as_OT.cmp_eq in E2. *)
+(*   all: subst*. *)
+(*   1: now rewrite* string_compare_refl. *)
+(*   1: now rewrite* E2. *)
+(*   1: now rewrite* E1. *)
+(*   Print NTTLB. *)
+(*   forwards: NTTLB.lt_trans s1 s2 s3. *)
+(*   unfolds. *)
+(*   all: try apply String_as_OT.cmp_lt in E1. *)
+(*   all: try apply String_as_OT.cmp_lt in E2. *)
+(*   all: try forwards H: String_as_OT.lt_trans E1 E2. *)
+(*   all: try rewrite <- String_as_OT.cmp_lt in H. *)
+(*   1: rewrite* H; simpl. *)
+
+(* Qed. *)
+
+(* no duplication sorted *)
+
+Definition sorted := Sorted lex_lt.
+
+Theorem sorted_unique : forall (l1 l2 : list string),
+    sorted l1 -> sorted l2 -> Permutation l1 l2 -> l1 = l2.
+Proof.
+  introv HS1 HS2 HP.
+  applys* Sort_In_eq lex_lt.
+  applys lex_lt_trans.
+  applys lex_lt_not_eq.
+  split; introv HI;
+    eauto using Permutation_sym, Permutation_in.
+Qed.
+
+Theorem merge_comm : forall (l1 l2 : list string),
+    sorted l1 -> sorted l2 ->
+    merge l1 l2 = merge l2 l1.
+    (* nodup string_dec (merge l1 l2) = nodup string_dec (merge l2 l1). *)
+Proof.
+  introv HS1 HS2.
+  applys* Sort_In_eq lex_lt.
+  admit.
+  applys lex_lt_not_eq.
+  admit. admit.
+  admit.
+  (* - lets HP: Permuted_merge. *)
+  (*   split; introv HI; applys nodup_In; apply nodup_In in HI; *)
+  (*     applys Permutation_in HP. *)
+  (*   all: applys in_app_iff; applys or_comm; applys in_app_iff. *)
+  (*   all: applys Permutation_in HI; applys* Permutation_sym HP. *)
+Admitted.
+
+(* Search Sorted. *)
+(* Admitted. *)
+(*   Search Permutation. *)
+(*   admit. admit. *)
+(*   - lets HP: Permuted_merge. *)
+(*     split; introv HI; applys nodup_In; apply nodup_In in HI; *)
+(*       applys Permutation_in HP. *)
+(*     all: applys in_app_iff; applys or_comm; applys in_app_iff. *)
+(*     all: applys Permutation_in HI; applys* Permutation_sym HP. *)
+(* Admitted. *)
+
+(*     nodup string_dec (merge l1 l2) = nodup string_dec (merge l3 ++ l4). *)
+
+Check Sorted_merge.
+
+Lemma In_merge : forall y l r,
+    In y (merge l r) <-> In y l \/ In y r.
+Proof.
+Admitted.
+
+(* Lemma HdRel_lt : forall a y l, *)
+(*     HdRel lex_lt a l -> In y l -> lex_lt a y. *)
+(* Proof with eauto with bool. *)
+(*   introv HR HI. gen a y. induction l; intros... *)
+(*   - inverts HI. *)
+(*   - Print HdRel. inverts HR. forwards: IHl H0. inverts HI. Print HdRel. *)
+(*   applys* SortA_InfA_InA l. 4: now applys* InA_iff_In. *)
+(*            eapply eq_equivalence. eapply lex_lt_strorder. *)
+(*            eapply NOTF.lt_compat. *)
+
+Lemma HdRel_nodup : forall a l,
+    Sorted NOTF.le l -> HdRel lex_lt a l -> HdRel lex_lt a (nodup string_dec l).
+Proof with eauto.
+  introv HS HR.
+  applys In_InfA. introv HI. apply nodup_In in HI.
+  induction l.
+  - inverts HI.
+  - apply in_inv in HI. destruct HI.
+    + subst*. inverts* HR.
+    + inverts HS. inverts HR.
+      forwards*: IHl.
+      inverts* H3. constructor.
+      destruct H0. now applys* lex_lt_trans.
+      now subst*.
+Qed.
+
+Lemma le_trans : forall s0 s1 s2 : string, NOTF.le s0 s1 -> NOTF.le s1 s2 -> NOTF.le s0 s2.
+Admitted.
+
+Lemma HdRel_nodup_le : forall a l,
+    Sorted NOTF.le l -> HdRel NOTF.le a l -> HdRel lex_lt a (nodup string_dec l).
+Proof with eauto.
+  introv HS HR. gen a. induction l; intros.
+  - simpl...
+  - inverts HS. inverts HR.
+    simpl. case_if*.
+    + applys* IHl.
+      inverts* H2. constructor...
+      eauto using le_trans.
+    + constructor...
+Abort. (* incorrect: a may be in l *)
+Check lex_lt_trans.  Check NTTLB.leb_trans.
+
+Lemma sorted_nodup_aux : forall l,
+    sorted (nodup string_dec l) -> Sorted NOTF.le l.
+Abort. (* incorrect *)
+
+Lemma sorted_nodup : forall l,
+    Sorted NOTF.le l -> sorted (nodup string_dec l).
+Proof with eauto.
+  introv HS. induction* l.
+  - simpl... econstructor...
+  - inverts HS. forwards*: IHl.
+    simpl. case_if.
+    + apply H.
+    + econstructor... destruct l...
+      * simpl...
+      * applys* HdRel_nodup.
+        inverts H2. inverts* H3.
+        exfalso. applys C. applys in_eq.
+Qed.
+
+(* Lemma HdRel_nodup : forall a l, *)
+(*         HdRel NOTF.le a l -> In b l -> lex_lt a b. *)
+(*         Search (Sorted). *)
+(*         inverts H2. inverts H3. econstructor. *)
+(*     fold nodup. *)
+(*     ; econstructor. *)
+(*     + forwards: IHl HS. constructor*. *)
+(*       clear HS IHl. *)
+(*       induction* l. *)
+(*       apply in_inv in C. destruct C. *)
+(*       * subst*. constructor*. right*. *)
+(*       * constructor. inverts H. *)
+(*         Search Sorted. *)
+
+
+(*         Search HdRel. applys* IHl. *)
+
+
+(*       Search (Sorted _ _ -> HdRel _ _ _). *)
+
+(*        HS : Sorted NOTF.le l *)
+(*   HR : HdRel lex_lt a l *)
+(*   y : string *)
+(*   HI : In y l *)
+(*   ============================ *)
+(*   lex_lt a y *)
+
+
+(*       Search (Sorted). *)
+
+Lemma HdRel_relax : forall a l,
+    HdRel lex_lt a l -> HdRel NOTF.le a l.
+Proof with eauto.
+  introv HS. induction* HS. constructor...
+  left*.
+Qed.
+
+Lemma sorted_relax : forall l,
+    sorted l -> Sorted NOTF.le l.
+Proof with eauto.
+  introv HS. induction* HS.
+  destruct H... constructor... constructor...
+  left*.
+Qed.
+
+#[local] Hint Constructors Sorted HdRel : core.
+#[local] Hint Resolve HdRel_relax sorted_relax : core.
+
+Lemma test : forall a l r,
+    HdRel NOTF.le a l -> HdRel NOTF.le a r -> HdRel NOTF.le a (merge l r).
+Admitted.
+
+Lemma merge_sorted : forall l r,
+    sorted l -> sorted r -> Sorted NOTF.le (merge l r).
+Proof with eauto using sorted_relax.
+  introv HSl HSr. gen r.
+  induction HSl; intros; autorewrite with merge...
+  - induction HSr...
+    + autorewrite with merge.
+      constructor...
+    + destruct (string_compare_lex a a0) eqn:HE. destruct c.
+      * subst*. simpl. rewrite HE. simpl...
+        econstructor. applys IHHSl...
+        econstructor... applys test...
+        econstructor... right*.
+      * simpl. rewrite HE. simpl...
+        forwards* IH: IHHSl (a0 :: l0)...
+        all: econstructor...
+        applys test...
+      * simpl. rewrite HE. simpl...
+        econstructor... applys test (a :: l) l0...
+Qed.
+
+Lemma merge_sorted_dedup: forall l r,
+    sorted l -> sorted r -> sorted (nodup string_dec (merge l r)).
+Proof with eauto using sorted_nodup, sorted_relax.
+  introv HSl HSr.
+  forwards: merge_sorted HSl HSr...
+Qed.
+(*   induction HSl; intros; autorewrite with merge... *)
+(*   - induction HSr... *)
+(*     + autorewrite with merge. simpl. case_if... *)
+(*       constructor... applys sorted_nodup... *)
+(*       applys HdRel_nodup... *)
+(*     + forwards* IH: IHHSl (a0 :: l0)... *)
+(*       econstructor... *)
+(*       simpl. case_if... simpl. case_if... *)
+(*       econstructor... applys HdRel_nodup... *)
+
+
+(*       econstructor... *)
+(*     + simpl. case_if*. *)
+(*       constructor*. applys* HdRel_nodup. applys* sorted_relax. *)
+(*   - induction HSr... *)
+(*     + autorewrite with merge. simpl. case_if... *)
+(* eauto using sorted_nodup *)
+(*     + autorewrite with merge. repeat case_if... *)
+(*       fold nodup.sorted_relax applys* SortA_InfA_InA. *)
+(*       sorted (nodup *)
+(*       autorewrite with merge. *)
+(*       constructor. *)
+(*     + forwards* HSP: IHHSl l0. *)
+(*       autorewrite with merge. case_if... *)
+(*       * case_if in C. forwards* HSP': IHHSl (a0 :: l0). *)
+(*         all: constructor... *)
+(*         applys In_InfA. introv HI. forwards [HI'|HI']: In_merge HI. *)
+(*         ** applys* SortA_InfA_InA l. 4: now applys* InA_iff_In. *)
+(*            eapply eq_equivalence. eapply lex_lt_strorder. *)
+(*            eapply NOTF.lt_compat. *)
+(*         ** applys* SortA_InfA_InA (a0 :: l0). 5: now applys* InA_iff_In. *)
+(*            eapply eq_equivalence. eapply lex_lt_strorder. *)
+(*            eapply NOTF.lt_compat. constructor... *)
+(*            Search (Proper (eq ==> eq ==> iff) lex_lt). *)
+(*         eauto. *)
+(*         Search (InA). *)
+(*         Search Sorted. *)
+(*         lets: InfA_app. *)
+(*         Search HdRel. SortA_InfA_InA. *)
+(*         case_if... *)
+(*       * case_if... *)
+(*         ** lets* HSP: IHHSl (y0 :: l0). forwards*: HSP. *)
+(*            case_if... *)
+(*         ** simpl in IHHSr. case_if... *)
+(* Qed. *)
+
+
+(* Theorem merge_comm : forall (l1 l2 : list string), *)
+(*   Sorted lex_lt l1 -> Sorted lex_lt l2 -> merge l1 l2 = merge l2 l1. *)
+(* Proof. *)
+(*   introv HS1 HS2. *)
+(*   lets: SortA_equivlistA_eqlistA. *)
+(*   Print StrictOrder. *)
+
+(*   Search (Sorted). *)
+(*   Search (lex_lt). *)
+(*   pose proof NTTLB.leb_trans. unfold Transitive in H. Print NOTF. Search le. *)
+(*   assert (forall x y, proj1_sig (string_compare_lex x y) = Lt -> *)
+(*                       lex_lt x y). eauto. *)
+(*   pose proof NOTF.compare_spec. intros. forwards: H0 x y. *)
+(*   destruct H2; try discriminate. eauto. *)
+(*   intros. destruct H1. destruct H2. Search NTTLB.leb. *)
+(*   Search CompareSpec. *)
+(*   NTTLB.leb_le: *)
+(*   forall x y : string, *)
+(*   is_true (NTTLB.leb x y) <-> (fun x0 y0 : string => lex_lt x0 y0 \/ x0 = y0) x y *)
+(* Admitted. *)
+
+(* } *)
+Open Scope string_scope.
+
+(* Properties of type translation *)
+Lemma foldl_append_singleton_list : forall T,
+    list_string_2_string [T] = T.
+Proof.
+  introv. simpl. eauto.
+Qed.
+
+Lemma check_toplike_sound_complete : forall A,
+    toplike A <-> check_toplike A = true.
+Proof.
+  split; introv HT.
+  - induction HT; simple*.
+    rewrite IHHT1. rewrite* IHHT2.
+  - induction* A.
+    all: simpl in HT; try discriminate.
+    forwards* (?&?): andb_prop_elim (check_toplike A1) (check_toplike A2).
+    eauto with bool.
+    constructor; intuition eauto using Is_true_eq_true.
+Qed.
+
+Lemma type2list_arrow : forall A B,
+  ~ toplike B ->
+  stype2string (typ_arrow A B) = [ ( "(" ++ (stype2string A) ++ "->" ++ (stype2string B) ++ ")" ) ].
+Proof.
+  introv NT.
+  simpl. case_if*. apply check_toplike_sound_complete in C. intuition eauto.
+Qed.
+
+Lemma index_arrow_inv : forall A B,
+    toplike B \/ || typ_arrow A B || = [ "(" ++ || A || ++ "->" ++ || B || ++ ")" ].
+Proof.
+  introv. destruct (check_toplike B) eqn:HE.
+  { left. applys* check_toplike_sound_complete. }
+  right. unfolds. simpl. case_if*.
+Qed.
+
+Lemma index_rcd_inv : forall l A,
+    toplike A \/ || typ_rcd l A || = [ "{" ++  l ++ "=>" ++ || A || ++ "}" ].
+Proof.
+  introv. destruct (check_toplike A) eqn:HE.
+  { left. applys* check_toplike_sound_complete. }
+  right. unfolds. simpl. case_if*.
+Qed.
+
+Lemma stype2string_toplike : forall A,
+    toplike A -> || A || = nil.
+Proof with eauto.
+  introv HT. apply check_toplike_sound_complete in HT.
+  destruct A; simpl in HT; try discriminate; simpl...
+  all: rewrite* HT.
+Qed.
+
+Lemma stype2string_and : forall A B : typ,
+    || typ_and A B || = nodup string_dec (merge (stype2string A) (stype2string B)).
+Proof.
+  introv. simpl.
+  destruct (check_toplike A) eqn:HA. destruct (check_toplike B) eqn:HB.
+  all: try apply check_toplike_sound_complete in HA.
+  all: try apply check_toplike_sound_complete in HB.
+  all: try ( rewrite (stype2string_toplike A); [ | eassumption] ).
+  all: try ( rewrite (stype2string_toplike B); [ | eassumption] ).
+  all: autorewrite with merge; simpl; eauto.
+Qed.
+
+
+Lemma eqIndTyp_toplike : forall A B,
+    eqIndTyp A B -> toplike A <-> toplike B.
+Proof with eauto.
+  introv HE. induction* HE.
+  all: try solve [split; intro H; intuition eauto].
+  all: try solve [split; intro H; econstructor; inverts H; intuition eauto].
+  all: try solve [split; intro H; econstructor; inverts H; try inverts H3; try inverts H2; intuition eauto].
+  all: try solve [split; intro H'; eauto; inverts H'; intuition eauto].
+Qed.
+
+(* Lemma test : forall A B, *)
+(*     ||A|| = ||B|| -> type2tlist A = type2tlist B. *)
+(* Proof with intuition eauto. *)
+(*   introv HE. unfold stype2string in HE. rewrite HE. *)
+Lemma typeindex_sorted: forall A,
+    sorted (|| A ||).
+Proof with eauto.
+  introv. induction* A; simpl...
+  all: unfolds...
+  all: try econstructor...
+  - case_if...
+    econstructor...
+  - case_if... applys* merge_sorted_dedup.
+  - case_if...
+    econstructor...
+Qed.
+
+Lemma typeindex_nodup: forall A,
+    NoDup (|| A ||).
+Proof with eauto.
+  introv. induction* A; simpl...
+Admitted.
+
+ Lemma merge_double_nodup : forall l,
+     nodup string_dec (merge l l) = nodup string_dec l.
+ Admitted.
+
+ Lemma typeindex_nodup_elim : forall A,
+     nodup string_dec (|| A ||) = || A ||.
+Proof with eauto.
+  introv. applys nodup_fixed_point. applys typeindex_nodup.
+Qed.
+
+#[local] Hint Rewrite typeindex_nodup_elim : merge.
+#[local] Hint Resolve typeindex_sorted : core.
+
+Lemma eqIndTyp_sound : forall A B,
+    eqIndTyp A B -> || A || = || B ||.
+Proof with eauto using typeindex_nodup, NoDup_nodup, merge_sorted_dedup.
+  introv HE. induction* HE.
+  - rewrite* IHHE1.
+  - lets [|]: index_arrow_inv A1 B1;
+      lets [|]: index_arrow_inv A2 B2.
+    2: forwards (HT2&?): eqIndTyp_toplike HE2;
+       forwards H': HT2 H.
+    3: forwards (?&HT2): eqIndTyp_toplike HE2;
+       forwards H': HT2 H0.
+    1-3: repeat rewrite stype2string_toplike...
+    rewrite H; rewrite H0; rewrite IHHE1; rewrite IHHE2...
+  - lets [|]: index_rcd_inv A;
+      lets [|]: index_rcd_inv B.
+    2: forwards (HT2&?): eqIndTyp_toplike HE;
+    forwards H': HT2 H.
+    3: forwards (?&HT2): eqIndTyp_toplike HE;
+    forwards H': HT2 H0.
+    1-3: repeat rewrite stype2string_toplike...
+    rewrite H; rewrite H0; rewrite IHHE...
+  - repeat rewrite stype2string_and. rewrite IHHE...
+  - repeat rewrite stype2string_and. rewrite* merge_comm.
+  - repeat rewrite stype2string_and.
+    applys sorted_unique...
+    applys* NoDup_Permutation... split; introv HI.
+    all: apply nodup_In; applys In_merge.
+    all: repeat apply nodup_In in HI; try apply In_merge in HI.
+    all: intuition eauto; repeat apply nodup_In in H; try apply In_merge in H; intuition eauto.
+    1-2: left; apply nodup_In; applys In_merge...
+    1-2: right; apply nodup_In; applys In_merge...
+  - rewrite stype2string_toplike...
+  - rewrite stype2string_and. rewrite stype2string_toplike...
+    autorewrite with merge...
+  - applys sorted_unique...
+    repeat rewrite stype2string_and.
+    rewrite IHHE.
+    applys* NoDup_Permutation... split; introv HI.
+    + rewrite* merge_double_nodup in HI.
+      rewrite* typeindex_nodup_elim in HI.
+    + rewrite* merge_double_nodup.
+      rewrite* typeindex_nodup_elim.
+      Unshelve. eauto.
+Qed.
+
+Lemma nodup_empty_inv : forall l,
+    nodup string_dec l = nil -> l = nil.
+Proof.
+  introv HE. induction* l.
+  simpl in HE. case_if.
+  exfalso. forwards~: IHl. subst. inverts C.
+Qed.
+
+Lemma merge_empty_inv : forall l r,
+    merge l r = nil -> l = nil /\ r = nil.
+Proof.
+  introv HE. destruct* l; destruct* r.
+  simpl in HE. case_if.
+Qed.
+
+Lemma stype2string_toplike_complete : forall A,
+    || A || = nil -> toplike A.
+Proof with eauto.
+  introv HT. apply check_toplike_sound_complete.
+  induction A; simpl in HT; try discriminate; try case_if; simpl...
+  apply nodup_empty_inv in HT.
+  forwards (?&?): merge_empty_inv HT.
+  forwards~: IHA1. forwards~: IHA2. rewrite H1. rewrite* H2.
+Qed.
+
+Lemma stype2string_single_and_inv : forall a A B,
+    [ a ] = || typ_and A B || -> ([ a ] = || A || \/ [ a ] = || B ||) /\ (nil = || A || \/ nil = || B ||).
+Proof with eauto using NoDup_nodup, merge_sorted_dedup, check_toplike_sound_complete.
+  introv HE.
+  rewrite stype2string_and in HE. gen a B.
+  induction (|| A ||); intros.
+  - autorewrite with merge in HE...
+  - Search nodup. induction (|| B ||).
+    + autorewrite with merge in HE...
+Admitted.
+
+Lemma eqIndTyp_complete : forall A B,
+    || A || = || B || -> eqIndTyp A B.
+Proof with eauto using NoDup_nodup, merge_sorted_dedup, check_toplike_sound_complete.
+  introv HE. gen B.
+  induction A; intros.
+  - forwards*: stype2string_toplike_complete B...
+  - simpl in HE. induction B...
+    all: try solve [simpl in HE; try case_if; try discriminate].
+    forwards ([|]&[|]): stype2string_single_and_inv HE.
+    all: try forwards: IHB1 H. all: try forwards: IHB1 H0.
+    admit.
+    forwards*: stype2string_toplike_complete B2...
+    applys EI_trans H1. applys EI_trans EI_comm.
+    applys EI_trans EI_and. applys EI_symm EI_topelim.
+    applys* EI_symm EI_top.
+    admit. admit.
+  - admit.
+  - admit.
+  - (* and case ??? : 1)either toplike 2) destruct B || normalize *) admit.
+  - admit.
+Admitted.
+
+Lemma eqIndTyp_sound_target : forall A B,
+    eqIndTyp A B -> eqIndTypTarget |[A]| |[B]|.
+Proof.
+  introv HE. induction HE.
+  - (* refl *) admit.
+  - (* trans *) admit.
+  - (* symm *) admit.
+  - (* arrow congurence *) admit.
+  - (* rcd; needs property about eqindtyp *)
+    simpl. case_if; case_if. 1-3: admit.
+    admit.
+  - (* list; needs property about eqindtyp ? *)
+    simpl. admit.
+  - (* list swap ? *) admit.
+  - (* assoc *) admit.
+  - apply check_toplike_sound_complete in H.
+    simpl. (* toplike |[ A ]| ttyp_top *) admit.
+  - admit.
+  - (* double *) admit.
+Admitted.
+
+(* after deduplication is the same permutation *)
+
+(*   flattern a tree to a list? *)
+
+(*   generate sets from list / tree? *)
+
+
+(*   f (A & B) = f(C) *)
+
+(*                 f(A) = f(B) --> |[ A ]| ~ |[ B ]| *)
+
+(*   label->type *)
+
+
+(*            (A & B) & C *)
+
+(*         \y. ( \x. (\r. A | r) (\r. B | r) x ) ((\r.C|r) y) *)
+
+Definition eqIndTyp A B := sub A B. (* forall C, sub A C -> sub B C. *)
+
+Lemma sub_andl_inv : forall A B C,
+    sub (typ_and A B) C <-> sub A C \/ sub B C.
+Admitted.
+
+
+Lemma eqIndTyp_complete_alt : forall A B,
+    || A || = || B || -> eqIndTyp A B.
+Proof with eauto using NoDup_nodup, merge_sorted_dedup, check_toplike_sound_complete.
+  introv HE. gen B.
+  induction A; intros.
+  - forwards*: stype2string_toplike_complete B... admit. (* toplike super top *)
+  - (* bot sub all *) admit.
+  - simpl in HE. induction B...
+    all: try solve [simpl in HE; try case_if; try discriminate].
+    + (* refl *) admit.
+    + forwards ([|]&[|]): stype2string_single_and_inv HE.
+      (* stype2string_toplike_complete *)
+      all: try forwards: IHB1 H. all: try forwards: IHB1 H0.
+      all: admit.
+      (* forwards*: stype2string_toplike_complete B2... *)
+      (* applys EI_trans H1. applys EI_trans EI_comm. *)
+      (* applys EI_trans EI_and. applys EI_symm EI_topelim. *)
+      (* applys* EI_symm EI_top. *)
+  - (* arrow *)
+    simpl in HE. case_if.
+    + admit.
+      (* stype2string_toplike_complete *)
+    + induction B...
+      all: try solve [simpl in HE; try case_if; try discriminate].
+      * (* arrow *)
+        simpl in HE. case_if.
+        injection HE. intro HEq.
+        Search (_ ++ _ = _ ++ _). (* better use an inductive type as a label *)
+        assert (|| A1 || = || B1 ||) by admit. assert (|| A2 || = || B2 ||) by admit.
+        forwards*: IHA1. forwards*: IHA2.
+        (* contravariant problem *)
+        Restart.
+Proof with eauto using NoDup_nodup, merge_sorted_dedup, check_toplike_sound_complete.
+  introv HE. indTypSize (size_typ A + size_typ B).
+  destruct A; intros.
+  - forwards*: stype2string_toplike_complete B... admit. (* toplike super top *)
+  - (* bot sub all *) admit.
+  - simpl in HE. destruct B...
+    all: try solve [simpl in HE; try case_if; try discriminate].
+    + (* refl *) admit.
+    + forwards ([|]&[|]): stype2string_single_and_inv HE.
+      (* stype2string_toplike_complete *)
+      all: try forwards: IHB1 H. all: try forwards: IHB1 H0.
+      all: admit.
+      (* forwards*: stype2string_toplike_complete B2... *)
+      (* applys EI_trans H1. applys EI_trans EI_comm. *)
+      (* applys EI_trans EI_and. applys EI_symm EI_topelim. *)
+      (* applys* EI_symm EI_top. *)
+  - (* arrow *)
+    simpl in HE. case_if.
+    + admit.
+      (* stype2string_toplike_complete *)
+    + induction B...
+      all: try solve [simpl in HE; try case_if; try discriminate].
+      * (* arrow *) clear IHB1 IHB2.
+        simpl in HE. case_if.
+        injection HE. intro HEq.
+        Search (_ ++ _ = _ ++ _). (* better use an inductive type as a label *)
+        assert (|| B1 || = || A1 ||) by admit. assert (|| A2 || = || B2 ||) by admit.
+        forwards*: IH H. elia. forwards*: IH H0. elia.
+        applys* S_arr.
+      * (* and *)
+        forwards ([|]&[|]): stype2string_single_and_inv HE.
+        simpl in HE. rewrite <- H0 in HE.
+        case_if in HE.
+        assert (Heq: nodup string_dec (syntax_ott.NSort.merge nil (|| B2 ||)) = || B2 ||) by admit.
+        rewrite Heq in HE. forwards: IHB2 HE. elia.
+        forwards*: stype2string_toplike_complete B1.
+        admit. admit. admit. admit.
+  - destruct B.
+    + admit. (* top *)
+    + admit. (* single *)
+    + admit. (* single *)
+    + admit. (* single *)
+    + (* prove (typ_and A1 A2) <: B1 *)
+      (* prove (typ_and A1 A2) <: B2 *)
+      assert (incl (|| A1 ||) (|| typ_and A1 A2 ||)).
+      assert (incl (|| A2 ||) (|| typ_and A1 A2 ||)).
+      all: admit.
+    + admit. (* single *)
+  - admit.
+Admitted.
+
+Lemma incl_single: forall (x y : string), incl [x] [y] -> x = y.
+Proof.
+        introv HI.
+        apply incl_Forall_in_iff in HI.
+        apply Forall_inv in HI.
+        apply in_one_iff in HI. eauto.
+Qed.
+Lemma incl_eq : forall (l1 l2 : list string), l1 = l2 -> incl l1 l2.
+Proof.
+  introv Heq. rewrite Heq. applys* incl_refl.
+Qed.
+
+Lemma eqIndTyp_complete_alt_gen : forall A B,
+    incl (|| B ||) (|| A ||) -> sub A B.
+Proof with eauto using NoDup_nodup, merge_sorted_dedup, check_toplike_sound_complete.
+  introv HE. indTypSize (size_typ A + size_typ B).
+  destruct A; intros.
+  - forwards*: stype2string_toplike_complete B... admit. (* toplike super top *)
+  - (* bot sub all *) eauto. admit.
+  - simpl in HE. Search incl. destruct B...
+    all: try solve [simpl in HE; try case_if; forwards: incl_single HE; try discriminate].
+    + simpl in HE. case_if. admit.
+      forwards: incl_single HE. discriminate.
+    + admit.
+    + admit.
+  - (* arrow *)
+    simpl in HE. case_if.
+    + admit.
+      (* stype2string_toplike_complete *)
+    + destruct B...
+      all: try solve [simpl in HE; try case_if; try discriminate].
+      3: {
+        (* arrow *)
+        simpl in HE. case_if. admit.
+        forwards: incl_single HE.
+        injection H. intro HEq.
+        Search (_ ++ _ = _ ++ _). (* better use an inductive type as a label *)
+        assert (|| B1 || = || A1 ||) by admit. assert (|| A2 || = || B2 ||) by admit.
+        forwards: IH B1 A1; eauto using incl_eq. elia.
+        forwards: IH A2 B2; eauto using incl_eq. elia.
+      }
+      3: { (* and *) admit.
+           (* forwards ([|]&[|]): stype2string_single_and_inv HE. *)
+           (* simpl in HE. rewrite <- H0 in HE. *)
+           (* case_if in HE. *)
+           (* assert (Heq: nodup string_dec (syntax_ott.NSort.merge nil (|| B2 ||)) = || B2 ||) by admit. *)
+           (* rewrite Heq in HE. forwards: IHB2 HE. elia. *)
+           (* forwards*: stype2string_toplike_complete B1. *)
+      }
+      admit. admit. admit.
+  - simpl in HE. case_if. admit.
+    assert (incl (nodup string_dec (syntax_ott.NSort.merge (|| A1 ||) (|| A2 ||))) ((|| A1 ||) ++ (|| A2 ||))). {
+      applys nodup_incl string_dec.
+      Search (incl). admit.
+    }
+    forwards: incl_tran HE H.
+  (*   + admit. (* top *) *)
+  (*   + admit. (* single *) *)
+  (*   + admit. (* single *) *)
+  (*   + admit. (* single *) *)
+  (*   + (* prove (typ_and A1 A2) <: B1 *) *)
+  (*     (* prove (typ_and A1 A2) <: B2 *) *)
+  (*     assert (incl (|| A1 ||) (|| typ_and A1 A2 ||)). *)
+  (*     assert (incl (|| A2 ||) (|| typ_and A1 A2 ||)). *)
+  (*     all: admit. *)
+  (*   + admit. (* single *) *)
+  (* - admit. *)
+    Restart.
+  introv HE. indTypSize (size_typ A + size_typ B).
+  destruct B; intros; eauto.
+  - simpl in HE.
+    apply incl_Forall_in_iff in HE.
+    apply Forall_inv in HE.
+    destruct A; simpl in HE; try solve [try case_if; try destruct HE; try discriminate; intuition eauto; inverts H].
+    + admit.
+    + case_if.
+       assert (incl (nodup string_dec (syntax_ott.NSort.merge (|| A1 ||) (|| A2 ||))) ((|| A1 ||) ++ (|| A2 ||))). {
+      applys nodup_incl string_dec.
+      Search (incl). admit.
+    }
+    forwards Hia: In_incl HE H.
+       forwards [|]: in_app_or Hia.
+       assert (incl (||typ_bot||) (||A1||)). admit.
+       forwards: IH H1. elia.
+       eauto.
+       admit.
+  - admit.
+  - simpl in HE; try case_if. admit.
+    try apply incl_Forall_in_iff in HE.
+    try apply Forall_inv in HE.
+    destruct A; simpl in HE; try solve [try case_if; try destruct HE; try discriminate; intuition eauto; inverts H].
+    + admit. (* arrow vs arrow *)
+    + (* similar *)
+      admit.
+  - assert (incl (|| B1 ||)(|| typ_and B1 B2 ||)). {
+      simpl. case_if. admit.
+      assert (incl ((|| B1 ||) ++ (|| B2 ||)) (syntax_ott.NSort.merge (|| B1 ||) (|| B2 ||))) by admit.
+      applys nodup_incl.
+      applys incl_tran H. applys incl_appl. applys incl_refl.
+    }
+    assert (incl (|| B2 ||)(|| typ_and B1 B2 ||)) by admit.
+    forwards: incl_tran H HE. forwards: incl_tran H0 HE.
+    forwards*: IH A B1. elia. forwards*: IH A B2. elia.
+  - admit.
+Admitted.
+
+(* (incl (nodup string_dec (syntax_ott.nsort.merge (|| a1 ||) (|| a2 ||))) ((|| a1 ||) ++ (|| a2 ||))) *)
+(* incl ((|| b1 ||) ++ (|| b2 ||)) (syntax_ott.nsort.merge (|| b1 ||) (|| b2 ||)) *)
+
+(* !! soundness hard to prove *)
+
+Print subtype_wrt_lookup.
+
+Definition lookup_none A B: forall l, Tlookup l A = None -> Tlookup l B = None.
+
+Definition subtype_wrt_lookup_relax At Bt :=
+  rec_typ At /\ rec_typ Bt /\ wf_typ At /\ wf_typ Bt /\ forall l B, Tlookup l Bt = Some B -> exists A, Tlookup l At = Some A /\ subtype_wrt_lookup_relax A B.
+
+Lemma eqind_sound_target : forall A B,
+    ||A|| = ||B|| -> subtype_wrt_lookup |[A]| |[B]|.
+Proof.
+  introv HE.
+  incl_eq
+  eqIndTyp_complete_alt_gen
+
+    - use sub to replace eqindex
+
+    new equality
+    A&B = C if tolist A ++ tolist B .. C
+
+                 1) manually prove; equality up to permutation
+                                      2)
+
+A < B
+      B < A
+            ---------------
+            A -> < B ->
