coq/coq/rules_inf2.v
@@ -15,18 +15,6 @@ Require Export syntax_ott.
 (* *********************************************************************** *)
 (** * Induction principles for nonterminals *)
 
-Scheme tindex_ind' := Induction for tindex Sort Prop.
-
-Definition tindex_mutind :=
-  fun H1 H2 H3 H4 H5 H6 =>
-  tindex_ind' H1 H2 H3 H4 H5 H6.
-
-Scheme tindex_rec' := Induction for tindex Sort Set.
-
-Definition tindex_mutrec :=
-  fun H1 H2 H3 H4 H5 H6 =>
-  tindex_rec' H1 H2 H3 H4 H5 H6.
-
 Scheme ttyp_ind' := Induction for ttyp Sort Prop.
 
 Definition ttyp_mutind :=
@@ -64,8 +52,8 @@ Fixpoint close_texp_wrt_texp_rec (n1 : nat) (x1 : var) (t1 : texp) {struct t1} :
     | texp_fixpoint t2 => texp_fixpoint (close_texp_wrt_texp_rec (S n1) x1 t2)
     | texp_app t2 t3 => texp_app (close_texp_wrt_texp_rec n1 x1 t2) (close_texp_wrt_texp_rec n1 x1 t3)
     | texp_nil => texp_nil
-    | texp_cons ll1 t2 t3 => texp_cons ll1 (close_texp_wrt_texp_rec n1 x1 t2) (close_texp_wrt_texp_rec n1 x1 t3)
-    | texp_proj t2 ll1 => texp_proj (close_texp_wrt_texp_rec n1 x1 t2) ll1
+    | texp_cons l1 t2 t3 => texp_cons l1 (close_texp_wrt_texp_rec n1 x1 t2) (close_texp_wrt_texp_rec n1 x1 t3)
+    | texp_proj t2 l1 => texp_proj (close_texp_wrt_texp_rec n1 x1 t2) l1
     | texp_concat t2 t3 => texp_concat (close_texp_wrt_texp_rec n1 x1 t2) (close_texp_wrt_texp_rec n1 x1 t3)
   end.
 
@@ -75,22 +63,13 @@ Definition close_texp_wrt_texp x1 t1 := close_texp_wrt_texp_rec 0 x1 t1.
 (* *********************************************************************** *)
 (** * Size *)
 
-Fixpoint size_tindex (T1 : tindex) {struct T1} : nat :=
-  match T1 with
-    | ti_base => 1
-    | ti_arrow T2 => 1 + (size_tindex T2)
-    | ti_rcd l1 T2 => 1 + (size_tindex T2)
-    | ti_and T2 T3 => 1 + (size_tindex T2) + (size_tindex T3)
-    | ti_string l1 => 1
-  end.
-
 Fixpoint size_ttyp (At1 : ttyp) {struct At1} : nat :=
   match At1 with
     | ttyp_top => 1
     | ttyp_bot => 1
     | ttyp_base => 1
     | ttyp_arrow At2 Bt1 => 1 + (size_ttyp At2) + (size_ttyp Bt1)
-    | ttyp_rcd ll1 At2 Bt1 => 1 + (size_tindex ll1) + (size_ttyp At2) + (size_ttyp Bt1)
+    | ttyp_rcd l1 At2 Bt1 => 1 + (size_ttyp At2) + (size_ttyp Bt1)
   end.
 
 Fixpoint size_texp (t1 : texp) {struct t1} : nat :=
@@ -102,8 +81,8 @@ Fixpoint size_texp (t1 : texp) {struct t1} : nat :=
     | texp_fixpoint t2 => 1 + (size_texp t2)
     | texp_app t2 t3 => 1 + (size_texp t2) + (size_texp t3)
     | texp_nil => 1
-    | texp_cons ll1 t2 t3 => 1 + (size_tindex ll1) + (size_texp t2) + (size_texp t3)
-    | texp_proj t2 ll1 => 1 + (size_texp t2) + (size_tindex ll1)
+    | texp_cons l1 t2 t3 => 1 + (size_texp t2) + (size_texp t3)
+    | texp_proj t2 l1 => 1 + (size_texp t2)
     | texp_concat t2 t3 => 1 + (size_texp t2) + (size_texp t3)
   end.
 
@@ -133,13 +112,13 @@ Inductive degree_texp_wrt_texp : nat -> texp -> Prop :=
     degree_texp_wrt_texp n1 (texp_app t1 t2)
   | degree_wrt_texp_texp_nil : forall n1,
     degree_texp_wrt_texp n1 (texp_nil)
-  | degree_wrt_texp_texp_cons : forall n1 ll1 t1 t2,
+  | degree_wrt_texp_texp_cons : forall n1 l1 t1 t2,
     degree_texp_wrt_texp n1 t1 ->
     degree_texp_wrt_texp n1 t2 ->
-    degree_texp_wrt_texp n1 (texp_cons ll1 t1 t2)
-  | degree_wrt_texp_texp_proj : forall n1 t1 ll1,
+    degree_texp_wrt_texp n1 (texp_cons l1 t1 t2)
+  | degree_wrt_texp_texp_proj : forall n1 t1 l1,
     degree_texp_wrt_texp n1 t1 ->
-    degree_texp_wrt_texp n1 (texp_proj t1 ll1)
+    degree_texp_wrt_texp n1 (texp_proj t1 l1)
   | degree_wrt_texp_texp_concat : forall n1 t1 t2,
     degree_texp_wrt_texp n1 t1 ->
     degree_texp_wrt_texp n1 t2 ->
@@ -174,13 +153,13 @@ Inductive lc_set_texp : texp -> Set :=
     lc_set_texp (texp_app t1 t2)
   | lc_set_texp_nil :
     lc_set_texp (texp_nil)
-  | lc_set_texp_cons : forall ll1 t1 t2,
+  | lc_set_texp_cons : forall l1 t1 t2,
     lc_set_texp t1 ->
     lc_set_texp t2 ->
-    lc_set_texp (texp_cons ll1 t1 t2)
-  | lc_set_texp_proj : forall t1 ll1,
+    lc_set_texp (texp_cons l1 t1 t2)
+  | lc_set_texp_proj : forall t1 l1,
     lc_set_texp t1 ->
-    lc_set_texp (texp_proj t1 ll1)
+    lc_set_texp (texp_proj t1 l1)
   | lc_set_texp_concat : forall t1 t2,
     lc_set_texp t1 ->
     lc_set_texp t2 ->
@@ -239,25 +218,6 @@ Ltac default_case_split ::=
 
 Ltac default_auto ::= auto with arith lngen; tauto.
 Ltac default_autorewrite ::= fail.
-
-(* begin hide *)
-
-Lemma size_tindex_min_mutual :
-(forall T1, 1 <= size_tindex T1).
-Proof.
-apply_mutual_ind tindex_mutind;
-default_simp.
-Qed.
-
-(* end hide *)
-
-Lemma size_tindex_min :
-forall T1, 1 <= size_tindex T1.
-Proof.
-pose proof size_tindex_min_mutual as H; intuition eauto.
-Qed.
-
-Hint Resolve size_tindex_min : lngen.
 
 (* begin hide *)
 
@@ -836,12 +796,6 @@ Qed.
 
 Hint Resolve lc_texp_of_degree : lngen.
 
-Ltac tindex_lc_exists_tac :=
-  repeat (match goal with
-            | H : _ |- _ =>
-              fail 1
-          end).
-
 Ltac ttyp_lc_exists_tac :=
   repeat (match goal with
             | H : _ |- _ =>
@@ -974,8 +928,7 @@ default_simp;
 try solve [assert False by default_simp; tauto];
 (* non-trivial cases *)
 constructor; default_simp;
-try first [apply lc_set_tindex_of_lc_tindex
- | apply lc_set_texp_of_lc_texp];
+try first [apply lc_set_texp_of_lc_texp];
 default_simp; eapply_first_lt_hyp;
 (* instantiate the size *)
 match goal with
